Support post state hash

EvmYul/EllipticCurvesPy/keccak.py
@@ -1,8 +1,10 @@
 from hash import keccak256
 from base_types import Bytes
 import sys
+
 fileName : Bytes = sys.argv[1]
-f = open("EvmYul/EllipticCurvesPy/keccakInput.txt", "r")
+f = open(fileName, "r")
 data = bytes.fromhex(f.read())
 r = keccak256(data)
-print(bytes.hex(r), end = '')
+print(bytes.hex(r), end = '')    
+f.close()
