EvmYul/Maps/StorageMap.lean
@@ -21,6 +21,8 @@ import Batteries.Data.RBMap
 import Mathlib.Data.Multiset.Sort
 
 import EvmYul.Wheels
+import EvmYul.State.TrieRoot
+import EvmYul.SpongeHash.Keccak256
 
 namespace EvmYul
 
@@ -33,6 +35,18 @@ def Storage.toFinmap (self : Storage) : Finmap (λ _ : UInt256 ↦ UInt256) :=
 
 def Storage.toEvmYulStorage (self : Storage) : EvmYul.Storage :=
   self.foldl (init := ∅) λ acc k v ↦ acc.insert (UInt256.ofNat k.1) v
+
+def toBlobs (pair : UInt256 × UInt256) : Option (String × String) := do
+  -- dbg_trace "serialing storage item"
+  let kec := KEC pair.1.toByteArray
+  let rlp ← RLP (.𝔹 (BE pair.2.toNat))
+  -- dbg_trace "done serialing storage item"
+  pure (EvmYul.toHex kec, EvmYul.toHex rlp)
+
+def computeTrieRoot (storage : Storage) : Option ByteArray :=
+  match Array.mapM toBlobs storage.1.toArray with
+    | none => .none
+    | some pairs => (ByteArray.ofBlob (blobComputeTrieRoot pairs)).toOption
 
 /--
 It does _not_ matter how this is implemented at all, this is used _exclusively_ for convenience.
