EvmYul/State/TrieRoot.lean
@@ -1,0 +1,13 @@
+import EvmYul.PerformIO
+import EvmYul.Wheels
+
+def blobComputeTrieRoot (ws : Array (String × String)) : String :=
+  totallySafePerformIO ∘ IO.Process.run <|
+    pythonCommandOfInput ws
+  where pythonCommandOfInput (ws : Array (String × String)) : IO.Process.SpawnArgs := {
+    cmd := "python3",
+    args :=
+      #["EvmYul/EllipticCurvesPy/trie_root.py"]
+        ++ #[ws.size.repr]
+        ++ (ws.map (λ (i, w) ↦ #[i, w])).join
+  }
